proved while hoare rule for itrees

tutorial/ImpHoare.v
@@ -149,9 +149,9 @@ Proof.
     rewrite H. setoid_rewrite bind_ret. apply Hc2. auto.
 Qed.
 
-Timeout 5 Definition app {A B : Type} (f : A -> B) (a : A) := f a.
+Definition app {A B : Type} (f : A -> B) (a : A) := f a.
 
-Definition run_state_itree {A S : Type} {E : Type -> Type} (m : stateT S (itree E) A ) (s : S) : itree E (S * A) :=
+Definition run_state_itree {A S : Type} {E : Type -> Type} (s : S) (m : stateT S (itree E) A )  : itree E (S * A) :=
   m s.
 
 Global Instance EqStateEq {S R: Type} {E : Type -> Type} : Equivalence (@state_eq E R S).
@@ -162,10 +162,27 @@ Proof.
   - unfold state_eq in *. rewrite H. auto.
 Qed.
 
-(*
-Global Instance run_state_proper {E : Type -> Type} {S R : Type} : 
-  Proper (@state_eq E S R ==> @eutt E (S * R) (S * R) eq) (@run_state_itree R S E ).
-*)
+
+Global Instance run_state_proper_eq_itree {E : Type -> Type} {S R : Type} {s : S} : 
+  Proper (@state_eq E S R ==> eq_itree eq) (@run_state_itree R S E s).
+Proof.
+  repeat intro. unfold run_state_itree. unfold state_eq in H. rewrite H. reflexivity.
+Qed.
+
+
+Global Instance run_state_proper_eutt {E : Type -> Type} {S R : Type} {s : S} : 
+  Proper (@state_eq E S R ==> eutt eq) (@run_state_itree R S E s).
+Proof.
+  repeat intro. unfold run_state_itree. unfold state_eq in H. rewrite H. reflexivity.
+Qed.
+
+Global Instance eutt_proper_under_interp_state 
+       {E F: Type -> Type} {S R : Type} {h : E ~> stateT S (itree F) } :
+  Proper (eq_itree eq ==> @state_eq F S R) (fun (t : itree E R) =>  interp_state h t).
+Proof.
+  repeat intro. 
+Admitted.
+
 (*
 Check (case_ (handle_map (V := value) pure_state ) ).
 
@@ -180,8 +197,7 @@ Section interp_state_eq_iter.
   Context (A B : Type).
   Context (g : A ->itree E (A + B) ).
   Context (a : A).
-
-  Set Default Timeout 10.
+  
 
   Lemma interp_state_eq_iter : state_eq (interp_state f (KTree.iter g a) )
                               (MonadIter_stateT0 _ _ (fun a0 => interp_state f (g a0)) a).
@@ -192,7 +208,67 @@ Section interp_state_eq_iter.
   Qed.
 
 End interp_state_eq_iter.
+Set Default Timeout 15.
 
+Global Instance proper_state_eq_iter {S: Type} : 
+  Proper (@state_eq Void S (unit + unit) ==> @state_eq Void S (unit) ) (fun body => @MonadIter_stateT0 Delay S _ _ unit unit (fun _ : unit => body) tt ). 
+Proof.
+  repeat intro.
+  unfold MonadIter_stateT0, Basics.iter, MonadIterDelay. eapply eq_itree_iter.
+  repeat intro. subst. destruct y0 as [s' [] ].
+  simpl. specialize (H s'). rewrite H. reflexivity.
+Qed.
+
+Lemma interp_state_bind_state : forall (E F : Type -> Type) (A B S : Type)
+                   (h : forall T : Type, E T -> S -> itree F (S * T) ) (t : itree E A)
+                   (k : A -> itree E B), 
+    state_eq (interp_state h (ITree.bind t k)) 
+             (bind (interp_state h t) (fun a => interp_state h (k a) ) ).
+
+Proof.
+  unfold state_eq. intros. eapply interp_state_bind.
+Qed.
+
+Definition state_eq2 {E : Type -> Type} {A B S : Type} (k1 k2 : A -> stateT S (itree E) B ) : Prop :=
+  forall a, state_eq (k1 a)  (k2 a).
+
+Lemma eq_itree_clo_bind {E : Type -> Type} {R1 R2 : Type} :
+  forall (RR : R1 -> R2 -> Prop) (U1 U2 : Type) (UU : U1 -> U2 -> Prop)
+         (t1 : itree E U1) (t2 : itree E U2)
+         (k1 : U1 -> itree E R1) (k2 : U2 -> itree E R2),
+    eq_itree UU t1 t2 -> 
+    (forall (u1 : U1) (u2 : U2), UU u1 u2 -> eq_itree RR (k1 u1) (k2 u2)  ) -> 
+    eq_itree RR (ITree.bind t1 k1) (ITree.bind t2 k2).
+Proof.
+  intros. generalize dependent t2. generalize dependent t1.
+  pcofix CIH. 
+  intros. pinversion H1; eauto.
+  - specialize (@itree_eta E U1 t1 ) as Hr1.
+    rewrite <- H2 in Hr1.
+    specialize (@itree_eta E U2 t2) as Hr2.
+    rewrite <- H in Hr2.  pfold. red. Admitted.
+
+
+
+Global Instance bind_state_eq2 {E : Type -> Type} {A B S : Type} {m : stateT S (itree E) A} : 
+  Proper (@state_eq2 E A B S ==> @state_eq E S B) (bind m).
+Proof.
+  repeat intro. unfold state_eq2, state_eq in H. cbn.
+  eapply eq_itree_clo_bind; try reflexivity. intros. subst.
+  destruct u2 as [s' a]. simpl. rewrite H. reflexivity.
+Qed.
+
+
+Lemma compile_while : forall (b : bexp) (c : com), 
+                             (denote_imp ( WHILE b DO c END )) ≈ MonadIter_stateT0 unit unit 
+                                         (fun _ : unit => bind (interp_imp (denote_bexp b)) 
+                                                               (fun b : bool => if b 
+                                                                         then bind (denote_imp c) (fun _ : unit => interp_imp (Ret (inl tt)) )  
+                                                                         else interp_imp (Ret (inr tt))) ) tt.
+Proof.
+  intros. simpl. unfold denote_imp. simpl. unfold while. unfold interp_imp at 1, interp_map at 1.
+  cbn. red. red. intros. symmetry.
+Abort.
 Lemma hoare_while : forall (c : com) (b : bexp) (P : env -> Prop),
     {{fun s => is_true b s /\ P s}} c {{ P  }} ->
     {{ P }} WHILE b DO c END {{ fun s => is_false b s /\ P s}}.
@@ -207,95 +283,303 @@ Proof.
   fold m in H1.
   assert (state_eq m m); try reflexivity.
   unfold m at 1 in H2.  rewrite interp_state_eq_iter in H2.
-
-  (*still need to figure out how to use this run state notion
-    to rewrite this monad you did 
-    ironically this really gets back to my old contention that interps need to be iter morphisms
-*)
-
-(*
-  eapply interp_state_iter in H2.
-  match goal with | H : interp_state ?h0 _ _ ≈ _ |- _ => set h0 as h end.
-  fold h in H1. unfold IFun in h.
-  set (run_state_map h (A := unit)) as rs.
-  assert (rs )
+  fold (run_state_itree s m) in H1. symmetry in H2. 
+  
+  setoid_rewrite H2 in H1.
+  
+  match goal with | H : run_state_itree s (_ _ _ (fun _ => ?e) tt) ≈ _  |- _ => set e as body end.
+  assert (state_eq body body); try reflexivity.
+  
+  unfold body in H3 at 2.
+  setoid_rewrite interp_bind in H3.
+  fold body in H1. setoid_rewrite interp_state_bind_state in H3.
   
 
-  (*run_state (m : stateT ... ) (s : S) : Delay A, prove properness, use interp_state_iter*)
+  match type of H3 with state_eq _ (bind (?h0 (?h1 ?bexp) ) 
+                                         (fun be => ?h2 (?h3 (
+                                   if _ 
+                                   then ?l else ?r) ))) => set h0 as hsb; set h1 as hib; fold hsb in H3; fold hib in H3; 
+                                                             set h2 as hsu; set h3 as hiu; fold hsu in H3; fold hiu in H3  end.
+  assert (Hse : state_eq2 
+                  (fun b: bool => hsu (hiu (if b 
+                                            then ITree.bind (denote_com c) (fun _ : unit => Ret (inl tt)) 
+                                            else Ret (inr tt))))
+                  (fun b : bool => if b 
+                                   then bind (interp_imp (denote_com c) )  (fun _ : unit => interp_imp (Ret (inl tt)) ) 
+                                   else interp_imp (Ret (inr tt) ) ) 
+ ).
+  {
+    intro b0. destruct b0; try reflexivity. unfold hsu, hiu. setoid_rewrite interp_bind. unfold interp_imp, interp_map. intro.
+    setoid_rewrite interp_state_bind. unfold bind. simpl. reflexivity.
+  }
+  rewrite Hse in H3. clear Hse.
 
-  
-  
-  match goal with | H : interp_state _ (?t0 ) _ ≈ _ |- _ => set t0 as t end.
-  assert (t ≈ t); try reflexivity. unfold t in H2 at 2.
-  
-  setoid_rewrite interp_iter in H1. rewrite interp_state_iter in H1.
-  setoid_rewrite interp_iter in H1.
+  (*once I fully push down interps in body I can rewrite in H1*)
+  eapply proper_state_eq_iter in H3; eauto. rewrite H3 in H1. clear H3. 
+  unfold run_state_itree in H1. unfold hsb, hib, hsu, hiu in H1.
+  clear hsb hib hsu hiu. clear H2 body m. rename H1 into Heutt.
+  rename H0 into Hres.
+  specialize (loop_invar_state env unit unit) as Hloop. unfold State in Hloop.
 
-  About interp_iter. setoid_rewrite interp_iter in H1.
-  Match type of H2 with _ ≈ _ (fun _ => ?t0 ) _ => set t0 as while_body end.
-  assert (while_body ≈ while_body); try reflexivity.
-  unfold while_body in H3 at 2. 
-  rewrite interp_bind in H3. fold while_body in H2.
-  match type of H3 with _ ≈ ?t => set t as t' end.
+  match type of Heutt with MonadIter_stateT0 unit unit ?g tt _ ≈ _ => set g as body end.
 
-  (*f (if b then x else y) = if b then f x else f y *)
-  (*need good ways to streamline this interpretation*)
-  match type of H3 with _ ≈ ITree.bind _ ?f => assert (eq2 f f) end; try reflexivity.
-  assert (eq2 (fun r : bool =>
-          interp (bimap handle_ImpState (id_ Void))
-            (if r
-             then ITree.bind (denote_com c) (fun _ : unit => Ret (inl tt))
-             else Ret (inr tt)))
-          (fun r : bool =>
-          
-            (if r
-             then interp (bimap handle_ImpState (id_ Void)) (ITree.bind (denote_com c) (fun _ : unit => Ret (inl tt)))
-             else interp (bimap handle_ImpState (id_ Void)) (Ret (inr tt))))).
-  rewrite H4 in H3.
-*)
-(*
-  
-  match goal with | H : context [KTree.iter (fun _ => ?body) _ ] |- _ => 
-   set body as while_body end. fold while_body in H1.
-  assert (while_body ≅ while_body); try reflexivity. 
-  match goal with | H : interp ?f _ _ ≈ _ |- _ => set f as f' end. fold f' in H1.
-  set (@interp_imp Void) as T. unfold interp_imp, interp_map, interp_state in T.
-  unfold handle_ImpState in T. unfold handle_map in T.
-  (*so apparently we interpret from impstateE into mapE and I don't like that
-  *)
-  
-  unfold while_body in H2. fold f' in H2. setoid_rewrite bind_ret in H2. unfold denote_com in H2.
-  specialize (@interp_imp_bind Void) as Hinterp. 
-  unfold interp_imp, interp_map, interp_state in Hinterp.
-  (*fold (@interp_imp Void _ (handle_map (id_ Void) ) ) in H2. *)
-  setoid_rewrite interp_imp_bind in H2.
-  unfold Basics.iter, MonadIter_stateT0 in H1.
-  (*this context is probably proper with eq_itree*)
+  split.
+  - set (fun (t : Delay (env * unit) ) => 
+           (exists s, t ≈ ret (s,tt) /\ is_false b s) \/ divergence t
+        ) as p.
+    set (fun (t : Delay (env * unit + env * unit)) =>
+           (exists s, (t ≈ ret (inl (s,tt)) ) \/ ((t ≈ ret (inr (s,tt)) /\ is_false b s)) )  \/ divergence t
+        ) as q.
+    assert (resp_eutt _ _ p) as Hp.
+    {
+      unfold p. unfold is_false, is_bool.
+      intros t1 t2 He. split; intro; basic_solve.
+      - left. exists s0.  split; auto. rewrite <- He. auto.
+      - rewrite He in H0. auto.
+      - left. exists s0. split; auto. rewrite He. auto.
+      - rewrite <- He in H0. auto.
+    }
+    assert (resp_eutt _ _ q) as Hq.
+    {
+      unfold q. unfold is_true, is_false, is_bool.
+      intros t1 t2 He. split; intros; basic_solve.
+      - left. exists s0. rewrite He in H0. auto.
+      - left. exists s0. rewrite He in H0. auto.
+      - rewrite He in H0. auto.
+      - left. exists s0. rewrite He. auto.
+      - left. exists s0. rewrite He. auto.
+      - rewrite <- He in H0. auto.
+    }
+   enough (p (Ret (s',tt) ) ).
+    {
+      unfold p in H0. basic_solve; auto. pinversion H0.
+    }
+    enough (p (CategoryOps.iter body tt s) ).
+    {
+      eapply Hp; try apply H0. unfold CategoryOps.iter, Iter_Kleisli, Basics.iter.
+      unfold body. symmetry. auto.
+    }
+    enough ((p \1/ divergence) (CategoryOps.iter body tt s) ).
+    {
+      destruct H0; auto. unfold p. auto.
+    }
+    specialize Hloop with (s := s) (p := p) (q := q).
+    eapply Hloop; eauto.
+    + unfold reassoc. unfold body. 
+      destruct (eutt_reta_or_div _ (interp_imp (denote_com c) s ) );
+      destruct (classic_bool b s); basic_solve.
+      *  do 4 red in H1. unfold interp_imp, interp_map in H1.
+         destruct a as [s'' [] ]. 
+         eapply Hq.
+         -- cbn. setoid_rewrite bind_bind. rewrite H1.
+            setoid_rewrite bind_ret. simpl.
+            setoid_rewrite bind_bind. rewrite <- H0.
+            tau_steps. reflexivity.
+         -- unfold q. left. exists s''. left. reflexivity.
+      * do 4 red in H1. unfold interp_imp, interp_map in H1.
+        destruct a as [s'' [] ].
+        eapply Hq.
+        -- cbn. rewrite H1. setoid_rewrite bind_bind. setoid_rewrite bind_ret.
+           simpl. tau_steps. reflexivity.
+        -- unfold q. left. exists s. right. split; auto. reflexivity.
+      * do 4 red in H1. unfold interp_imp, interp_map in H1.
+        eapply Hq.
+        -- cbn. rewrite H1. setoid_rewrite bind_bind. setoid_rewrite bind_ret.
+           simpl. apply div_spin_eutt in H0. rewrite H0. setoid_rewrite bind_bind.
+           rewrite <- spin_bind. reflexivity.
+        -- red. right. apply spin_div.
+      * do 4 red in H1. unfold interp_imp, interp_map in H1.
+        eapply Hq.
+        -- cbn. rewrite H1. setoid_rewrite bind_bind. setoid_rewrite bind_ret.
+           simpl. apply div_spin_eutt in H0. 
+           tau_steps. reflexivity.
+        -- red. left. exists s. right. split; auto; reflexivity.
+   + unfold q,p. unfold DelaySpecMonad.loop_invar_imp. intros.
+     basic_solve.
+     * cbn in H0. exfalso. destruct (eutt_reta_or_div _ t); basic_solve.
+       -- rewrite <- H1 in H0. setoid_rewrite bind_ret in H0. basic_solve.
+       -- apply div_spin_eutt in H1. rewrite H1 in H0. rewrite <- spin_bind in H0.
+          symmetry in H0. eapply not_ret_eutt_spin; eauto.
+     * cbn in H0. destruct (eutt_reta_or_div _ t); basic_solve; auto.
+       rewrite <- H2 in H0. setoid_rewrite bind_ret in H0. basic_solve. left.
+       exists s0. split; auto. symmetry. auto.
+     * right. destruct (eutt_reta_or_div _ t); basic_solve; auto.
+       cbn in H0. rewrite <- H1 in H0. setoid_rewrite bind_ret in H0.
+       pinversion H0.
+  + unfold q. 
+    (*I chose the wrong q*)
 
-  match goal with | H : Basics.iter ?g ?a  ≈ _ |- _ => set g as g'; set a as a' end. 
-
-  fold g' in H1. fold a' in H1.
-  set (iter_arrow_rel g') as rg'.
-  destruct (classic_wf _ rg' a').
-  - unfold a' in H2. induction H2.
-    + unfold rg' in H2. unfold iter_arrow_rel in H2.
-      setoid_rewrite unfold_iter_ktree in H1.
-      destruct (eutt_reta_or_div _ (g' a) ); basic_solve.
-      * symmetry in H3. exfalso. eapply H2; eauto.
-      * destruct b0 as [s'' [] ]. rewrite <- H3 in H1.
-        setoid_rewrite bind_ret in H1. basic_solve.
-        unfold g' in H3.
-        destruct a as [s'' t]. simpl in *.
-        destruct (observe t) eqn : Heq.
-        -- setoid_rewrite bind_ret in H3. simpl in *.
+    unfold DelaySpecMonad.iter_lift, iso_destatify_arrow, reassoc. 
+    basic_solve; try (destruct (classic_bool b s0) ); 
+      try (destruct (eutt_reta_or_div _ (interp_imp (denote_com c) s0 ) )); basic_solve.
+    * eapply Hq.
+      -- cbn. rewrite H0. setoid_rewrite bind_ret.
+         setoid_rewrite bind_bind. do 4 red in H1. unfold interp_imp, interp_map in H1.
+         rewrite H1. setoid_rewrite bind_ret. simpl.
+         destruct a as [s1 [] ]. rewrite <- H2. setoid_rewrite bind_bind.
+         setoid_rewrite bind_ret. simpl. tau_steps. reflexivity.
+      -- red. left. destruct a as [s'' [] ]. exists s''. left. reflexivity.
+    * eapply Hq.
+      -- cbn. rewrite H0. setoid_rewrite bind_ret. setoid_rewrite bind_bind.
+         do 4 red in H1. unfold interp_imp, interp_map in H1. rewrite H1.
+         setoid_rewrite bind_ret. simpl. apply div_spin_eutt in H2. rewrite H2.
+         setoid_rewrite bind_bind. rewrite <- spin_bind. reflexivity.
+      -- right. apply spin_div.
+    * destruct a as [s'' [] ]. eapply Hq.
+      -- cbn.  rewrite H0. setoid_rewrite bind_ret.
+         do 4 red in H1. unfold interp_imp, interp_map in H1. rewrite H1.
+         setoid_rewrite bind_bind. setoid_rewrite bind_ret. simpl. tau_steps. reflexivity.
+      -- left. exists s0. right. split; auto. reflexivity.
+    * eapply Hq.
+      -- cbn.  rewrite H0. setoid_rewrite bind_ret.
+         do 4 red in H1. unfold interp_imp, interp_map in H1. rewrite H1.
+         setoid_rewrite bind_bind. setoid_rewrite bind_ret. simpl. tau_steps. reflexivity.
+      -- left. exists s0. right. split; auto. reflexivity.
+    * do 4 red in H1. do 4 red in H2. rewrite H1 in H2.
+      apply inv_ret in H2. injection H2. discriminate.
+    * do 4 red in H1. do 4 red in H2. rewrite H1 in H2.
+      apply inv_ret in H2. injection H2. discriminate.
+    * eapply Hq.
+      -- cbn.  rewrite H0. setoid_rewrite bind_ret.  reflexivity.
+      -- left. exists s0. right. split; auto. reflexivity.
+    * eapply Hq.
+      -- cbn.  rewrite H0. setoid_rewrite bind_ret.  reflexivity.
+      -- left. exists s0. right. split; auto. reflexivity.
+    * right. cbn. apply div_spin_eutt in H0. rewrite H0. rewrite <- spin_bind.
+      apply spin_div.
+   - set (fun (t : Delay (env * unit)) => 
+           (exists s, t ≈ ret (s,tt) /\ P s ) \/ divergence t
+        ) as p.
+    set (fun (t : Delay (env * unit + env * unit)) => 
+           (exists s, (t ≈ ret (inl (s,tt) ) \/ t ≈ ret (inr (s,tt) ) ) /\ P s )\/ divergence t )  as q.
+    assert (resp_eutt _ _ p) as Hp.
+    {
+      unfold p. intros t1 t2 He. split; intros; basic_solve.
+      - left. exists s0. rewrite He in H0. auto.
+      - right. rewrite He in H0. auto.
+      - left.  exists s0. rewrite <- He in H0. split; auto.
+      - right. rewrite He. auto.
+    }
+      assert (resp_eutt _ _ q) as Hq.
+      {
+        unfold q. intros t1 t2 He. split; intros; basic_solve.
+        - left. exists s0. rewrite He in H0. auto.
+        - left. exists s0. rewrite He in H0. auto.
+        - right. rewrite He in H0. auto. 
+        - left. rewrite <- He in H0. exists s0. auto.
+        - left. rewrite <- He in H0. exists s0. auto.
+        - right. rewrite He. auto.
+      }
+      specialize Hloop with (s := s) (p := p) (q := q).
+      
+      enough (p (Ret (s',tt))).
+      {
+        unfold p in H0. basic_solve; auto. pinversion H0.
+      }
+      enough ((p \1/ divergence) (CategoryOps.iter body tt s ) ).
+      { 
+        destruct H0.
+        - eapply Hp; try apply H0. rewrite <- Heutt. reflexivity.
+        - unfold CategoryOps.iter, Iter_Kleisli, Basics.iter in H0.
+          unfold body in H0. rewrite Heutt in H0. pinversion H0.
+      }
+      eapply Hloop; eauto.
+      + unfold reassoc. unfold body. destruct (classic_bool b s).
+        * assert (is_true b s /\ P s); auto. 
+          destruct (eutt_reta_or_div _ (interp_imp (denote_com c) s) ); basic_solve.
+          -- destruct a as [s'' [] ].
+             unfold is_true, is_bool in H0. 
+             unfold interp_imp, interp_map in H0.
+             eapply Hq.
+             ++ cbn. setoid_rewrite bind_bind. rewrite H0.
+                setoid_rewrite bind_ret. simpl. setoid_rewrite bind_bind.
+                rewrite <- H2. tau_steps.
+                reflexivity.
+             ++ specialize (H s s''). unfold q. left. exists s''. split; try (left; reflexivity).
+                eapply H; eauto. symmetry. auto.
+          -- apply div_spin_eutt in H2. eapply Hq with (t1 := spin).
+             ++ cbn. unfold is_true, is_bool in H0. setoid_rewrite bind_bind.
+                unfold interp_imp, interp_map in H0.  rewrite H0.
+                setoid_rewrite bind_ret. simpl. rewrite H2.
+                setoid_rewrite bind_bind. apply spin_bind.
+             ++ unfold q. right. apply spin_div.
+        * unfold is_false, is_bool, interp_imp, interp_map in H0. cbn.
+          eapply Hq.
+          -- setoid_rewrite bind_bind. rewrite H0. setoid_rewrite bind_ret.
+             simpl. cbn. tau_steps. reflexivity.
+          -- unfold q. left. exists s. split; auto. right. reflexivity.
+      + red. intros. unfold p. unfold q in H0. basic_solve.
+        * cbn in H0. 
+          destruct (eutt_reta_or_div _ t); basic_solve.
+          -- destruct a as [s'' [] ]. rewrite <- H2 in H0.
+             setoid_rewrite bind_ret in H0. basic_solve.
+          -- exfalso. apply div_spin_eutt in H2. rewrite H2 in H0. rewrite <- spin_bind in H0.
+             symmetry in H0. apply not_ret_eutt_spin in H0. auto.
+        * cbn in H0.
+        destruct (eutt_reta_or_div _ t); basic_solve.
+        -- destruct a as [s'' [] ]. rewrite <- H2 in H0.
+           setoid_rewrite bind_ret in H0. basic_solve. left. exists s0. 
+           symmetry in H2. auto.
+        -- exfalso. apply div_spin_eutt in H2. rewrite H2 in H0.
+           rewrite <- spin_bind in H0. symmetry in H0. apply not_ret_eutt_spin in H0. auto.
+      * cbn in H0. right. destruct (eutt_reta_or_div _ t); auto.
+        basic_solve. rewrite <- H1 in H0. setoid_rewrite bind_ret in H0.
+        pinversion H0.
+    + unfold DelaySpecMonad.iter_lift, iso_destatify_arrow, reassoc.
+      intros t Ht. cbn.
+      destruct (eutt_reta_or_div _ t); 
+         basic_solve.
+      * destruct a as [s'' [] ].
+        destruct (classic_bool b s''); 
+          destruct (eutt_reta_or_div _ (interp_imp (denote_com c) s'' )); basic_solve;
+        eapply Hq.
+        -- rewrite <- H0. setoid_rewrite bind_ret.
+           setoid_rewrite bind_bind. do 4 red in H1. 
+           unfold interp_imp, interp_map in H1. rewrite H1. setoid_rewrite bind_ret.
+           simpl. setoid_rewrite bind_bind.
+           rewrite <- H2. setoid_rewrite bind_ret. destruct a as [s3 [] ].
+           simpl. tau_steps. reflexivity.
+        -- destruct a as [s3 [] ]. unfold q in Ht. basic_solve.
+           ++ rewrite  H3 in H0. basic_solve.
+              unfold q. left. exists s3. split; try (left; reflexivity). symmetry in H2.
+              eapply H; eauto.
+           ++ rewrite H3 in H0. basic_solve.
+           ++ rewrite <- H0 in H3. pinversion H3.
+        -- rewrite <- H0. setoid_rewrite bind_ret. setoid_rewrite bind_bind.
+           do 4 red in H1. unfold interp_imp, interp_map in H1. rewrite H1.
+           setoid_rewrite bind_ret. simpl. apply div_spin_eutt in H2.
+           setoid_rewrite bind_bind. rewrite H2.
+           rewrite <- spin_bind. reflexivity.
+        -- unfold q. right. apply spin_div.
+        -- rewrite <- H0. setoid_rewrite bind_ret. 
+           unfold is_false, is_bool in H1. unfold interp_imp, interp_map in H1.
+           rewrite H1. setoid_rewrite bind_bind. setoid_rewrite bind_ret. simpl.
+           tau_steps. reflexivity.
+        -- unfold q. left. exists s''. split; try (right; reflexivity). unfold q in Ht.
            basic_solve.
-        
-  - apply iter_inl_spin in H2. rewrite H2 in H1. symmetry in H1.
-    exfalso.
-    eapply not_ret_eutt_spin.  eauto.
-  (*probably need to induce that arrow relation again*)
-  (*invariant is something that has a few cases*)
-  (*does burn preserve eutt? if so maybe write a tactic that just
-    runs a tactic a bunch*) *) Abort.
+           ++ rewrite H3 in H0. basic_solve. auto.
+           ++ rewrite H3 in H0. basic_solve.
+           ++ rewrite <- H0 in H3. pinversion H3.
+        -- rewrite <- H0. setoid_rewrite bind_ret. 
+           setoid_rewrite bind_bind.
+           do 4 red in H1. unfold interp_imp, interp_map in H1.
+           rewrite H1. setoid_rewrite bind_ret. simpl. tau_steps.
+           reflexivity.
+        -- unfold q. left. exists s''.
+           split; try (right; reflexivity). unfold q in Ht.
+           basic_solve.
+           ++ rewrite H3 in H0. basic_solve. auto.
+           ++ rewrite H3 in H0. basic_solve.
+           ++ rewrite <- H0 in H3. pinversion H3.
+     * destruct b0 as [s'' [] ]. eapply Hq.
+       -- rewrite <- H0. setoid_rewrite bind_ret.
+          reflexivity.
+       -- unfold q. left. exists s''. split; try (right; reflexivity).
+          unfold q in Ht. basic_solve.
+          ++ rewrite H1 in H0. basic_solve.
+          ++ rewrite H1 in H0. basic_solve. auto.
+          ++ rewrite <- H0 in H1. pinversion H1.
+     * clear Ht. unfold q. right. apply div_spin_eutt in H0.
+       rewrite H0. rewrite <- spin_bind. apply spin_div.
 
-  
+Qed.       
